VerificationSetCover/VerificationSetCover_simple.dfy
@@ -3,31 +3,40 @@ include "../Auxiliary/Lemmas.dfy"
 
 
 method verifySetCover(U:set<int>, S:set<set<int>>, k:nat, I:set<set<int>>) returns (b:bool, ghost counter:nat)   
-  requires forall s | s in S :: s <= U 
+  requires forall s | s in S :: s <= U
+  requires k <= |S|
+  requires forall i | i in I :: |i| <= |U|
   ensures b == (I <= S && isCover(U, I) && |I| <= k)
-  ensures counter <= poly(U, S, k, I)
+  ensures counter <= poly(U, S, k)
 {
   counter := 0;
   var U' := U; counter := counter + |U|;
   b:= true;
+  counter := counter + 1;
+  if (k < |I|) {
+    return false, counter;
+  }
   var I_seq_S:bool;
   I_seq_S, counter := isSubset(U, I, S, counter);
-  
-  counter := counter + 1;
-  if (!(I_seq_S && |I| <= k)) {
-    assert counter <= poly_isSubset(U, I, S) + |U| + 1;
+
+  if (!I_seq_S) {
+    assert counter <= |U| + 1 + poly_isSubset(U, I, S);
+    counter_simplification_special_case(U, S, k, I);
+    assert counter <= poly(U, S, k);
     return false, counter;
   }
   while (U' != {} && b)
     decreases |U'|
     invariant U' <= U 
     invariant b == isCover(U-U',I)
-    invariant counter <= |U| + poly_isSubset(U, I, S) + 1 + (|U| - |U'|)*(poly_outer_loop(U, S, k, I) + 1)
+    invariant counter <= |U| + poly_isSubset(U, I, S) + 1 + (|U| - |U'|)*(poly_outer_loop(U, S, k) + 1)
   {
     counter := counter + 1;
     b, U', counter := verifySetCover_outer_loop(U, S, k, I, U', counter);
   }
   counter := counter + 1;
+  assert counter <= |U| + poly_isSubset(U, I, S) + 2 + |U|*(poly_outer_loop(U, S, k) + 1);
+  counter_simplification(U, S, k, I);
   assert b ==> U-U' == U;
 }
 
@@ -84,30 +93,33 @@ method verifySetCover_outer_loop(U:set<int>, S:set<set<int>>, k:nat, I:set<set<i
   // Invariant in
   requires U' <= U
   requires isCover(U - U', I)
+  requires |I| <= |S|
   // Termination out
   ensures |U''| == |U'| - 1
   // Invariant out
   ensures U'' <= U
   ensures b1 == isCover(U - U'', I)
   // Counter
-  ensures counter <= counter_in + poly_outer_loop(U, S, k, I)
+  ensures counter <= counter_in + poly_outer_loop(U, S, k)
 {
   counter := counter_in;
   var u :| u in U'; counter := counter + 1;
   U'' := U' - {u}; counter := counter + |U|;
 
-  var I' := I; counter := counter + |I|;      // |S|*|U|
+  var I' := I; counter := counter + |S|*|U|;
   b1:= false;
   while (I' != {} && !b1)
     decreases |I'|
     invariant I' <= I
     invariant b1 == (exists i' | i' in I - I' :: u in i')
-    invariant counter == counter_in + |I| + |U| + 1 + (|I|-|I'|)*(poly_inner_loop(U, S, k, I) + 1)
+    invariant counter <= counter_in + |S|*|U| + |U| + 1 + (|I|-|I'|)*(poly_inner_loop(U, S, k) + 1)
   {
     counter := counter + 1;
     b1, I', counter := verifySetCover_inner_loop(U, S, k, I, I', u, counter);
   }
   counter := counter + 1;
+  assert counter <= counter_in + |S|*|U| + |U| + 2 + (|I|-|I'|)*(poly_inner_loop(U, S, k) + 1);
+  assert counter <= counter_in + |S|*|U| + |U| + 2 + (|S|)*(poly_inner_loop(U, S, k) + 1);
   assert U - U'' == U - U' + {u};
 }
 
@@ -124,12 +136,12 @@ method verifySetCover_inner_loop(U:set<int>, S:set<set<int>>, k:nat, I:set<set<i
   ensures I'' <= I
   ensures b2 == (exists i' | i' in I - I'' :: u in i')
   // Counter
-  ensures counter == counter_in + poly_inner_loop(U, S, k, I)
+  ensures counter == counter_in + poly_inner_loop(U, S, k)
 {
   counter := counter_in;
-  var i :| i in I'; counter := counter + |I|;     // |U|
-  b2 := u in i; counter := counter + |I|;         // |U|
-  I'' := I' - {i}; counter := counter + |I|;      // |S|*|U|
+  var i :| i in I'; counter := counter + |U|;
+  b2 := u in i; counter := counter + |U|;
+  I'' := I' - {i}; counter := counter + |S|*|U|;
 }
 
 
@@ -141,27 +153,28 @@ ghost function poly_isSubset(U: set<int>, S1:set<set<int>>, S2:set<set<int>>) : 
 {
   |S1|*|S1|*|U| + |S1|*|S2|*|U| + 2*|S1|*|U| + |S1| + 2
 }
-ghost function poly_inner_loop(U: set<int>, S: set<set<int>>, k: nat, I:set<set<int>>) : (o:nat) {
-  //|S|*|U| + 2*|U|
-  3*|I|
+ghost function poly_inner_loop(U: set<int>, S: set<set<int>>, k: nat) : (o:nat) {
+  |S|*|U| + 2*|U|
 }
-ghost function poly_outer_loop(U: set<int>, S: set<set<int>>, k: nat, I:set<set<int>>) : (o:nat)
-  ensures |I| + |U| + 2 + |I|*(3*|I| + 1) == o
+ghost function poly_outer_loop(U: set<int>, S: set<set<int>>, k: nat) : (o:nat)
+  ensures |S|*|U| + |U| + 2 + |S|*(poly_inner_loop(U, S, k) + 1) == o
 {
-  3*|I|*|I| + 2*|I| + |U| + 2
+  |U|*|S|*|S| + 3*|U|*|S| + |U| + |S| + 2
 }
 
 
-ghost function poly(U: set<int>, S: set<set<int>>, k: nat, I:set<set<int>>) : (o:nat)
-  ensures poly_isSubset(U, I, S) + |U| + 1 <= o 
-  ensures |U| + poly_isSubset(U, I, S) + 2 + |U|*(poly_outer_loop(U, S, k, I) + 1) <= o
+ghost function poly(U: set<int>, S: set<set<int>>, k: nat) : (o:nat)
+  //ensures poly_isSubset(U, I, S) + |U| + 1 <= o 
+  //ensures |U| + poly_isSubset(U, I, S) + 2 + |U|*(poly_outer_loop(U, S, k, I) + 1) <= o
 {
+  /*
   calc <= {
     poly_isSubset(U, I, S) + |U| + 1;
     |I|*|I|*|U| + |I|*|S|*|U| + 2*|I|*|U| + |I| + |U| + 3;
     4*|I|*|I|*|U| + |I|*|S|*|U| + 4*|I|*|U| + |U|*|U| + |I| + 4*|U| + 4;
+    5*|S|*|S|*|U| + 4*|S|*|U| + |U|*|U| + 4*|U| + |S| + 4;
   }
-  /*
+  
   calc <= {
     |U| + poly_isSubset(U, I, S) + 2 + |U|*(poly_outer_loop(U, S, k, I) + 1);
     |U| + poly_isSubset(U, I, S) + 2 + |U|*poly_outer_loop(U, S, k, I) + |U|;
@@ -170,7 +183,64 @@ ghost function poly(U: set<int>, S: set<set<int>>, k: nat, I:set<set<int>>) : (o
     |I|*|I|*|U| + |I|*|S|*|U| + 2*|I|*|U| + |I| + 2*|U| + 4 + |U|*(3*|I|*|I| + 2*|I| + |U| + 2);
     |I|*|I|*|U| + |I|*|S|*|U| + 2*|I|*|U| + |I| + 2*|U| + 4 + 3*|I|*|I|*|U| + 2*|I|*|U| + |U|*|U| + 2*|U|;
     4*|I|*|I|*|U| + |I|*|S|*|U| + 4*|I|*|U| + |U|*|U| + |I| + 4*|U| + 4;
+    5*|S|*|S|*|U| + 4*|S|*|U| + |U|*|U| + 4*|U| + |S| + 4;
+  }*/
+  
+  // 4*|I|*|I|*|U| + |I|*|S|*|U| + 4*|I|*|U| + |U|*|U| + |I| + 4*|U| + 4
+  |S|*|S|*|U|*|U| + 2*|S|*|S|*|U| + 3*|S|*|U|*|U| + 3*|S|*|U| + |U|*|U| + |S| + 4*|U| + 4
+}
+
+
+lemma counter_simplification(U: set<int>, S: set<set<int>>, k: nat, I: set<set<int>>)
+  requires |I| <= |S|
+  ensures |U| + poly_isSubset(U, I, S) + 2 + |U|*(poly_outer_loop(U, S, k) + 1) <= poly(U, S, k)
+{
+  calc <= {
+    |U| + poly_isSubset(U, I, S) + 2 + |U|*(poly_outer_loop(U, S, k) + 1);
+    |U| + |I|*|I|*|U| + |I|*|S|*|U| + 2*|I|*|U| + |I| + |U|*(poly_outer_loop(U, S, k) + 1) + 4;
+    |I|*|I|*|U| + |I|*|S|*|U| + 2*|I|*|U| + |I| + 2*|U| + 4 + |U|*poly_outer_loop(U, S, k);
+    |I|*|I|*|U| + |I|*|S|*|U| + 2*|I|*|U| + |I| + 2*|U| + 4 + (|S|*|S|*|U|*|U| + 3*|S|*|U|*|U| + |U|*|U| + |S|*|U| + 2*|U|);
+    assert 2*|I|*|U| <= 2*|S|*|U| by {
+      mult_preserves_order(|I|, 2*|U|, |S|, 2*|U|);
+    }
+    |I|*|I|*|U| + |I|*|S|*|U| + 2*|S|*|U| + |S|*|S|*|U|*|U| + 3*|S|*|U|*|U| + |U|*|U| + |S|*|U| + |S| + 4*|U| + 4;
+    assert |I|*|I|*|U| <= |I|*|S|*|U| by {
+      mult_preserves_order(|I|, |I|*|U|, |S|, |I|*|U|);
+      assert |I|*|I|*|U| <= |S|*|I|*|U|;
+      assert |S|*|I|*|U| <= |I|*|S|*|U|;
+    }
+    |I|*|S|*|U| + |I|*|S|*|U| + 2*|S|*|U| + |S|*|S|*|U|*|U| + 3*|S|*|U|*|U| + |U|*|U| + |S|*|U| + |S| + 4*|U| + 4;
+    2*|I|*|S|*|U| + 2*|S|*|U| + |S|*|S|*|U|*|U| + 3*|S|*|U|*|U| + |U|*|U| + |S|*|U| + |S| + 4*|U| + 4;
+    assert |I|*|S|*|U| <= |S|*|S|*|U| by {
+      mult_preserves_order(|I|, |S|*|U|, |S|, |S|*|U|);
+    }
+    2*|S|*|S|*|U| + 2*|S|*|U| + |S|*|S|*|U|*|U| + 3*|S|*|U|*|U| + |U|*|U| + |S|*|U| + |S| + 4*|U| + 4;
+    |S|*|S|*|U|*|U| + 2*|S|*|S|*|U| + 3*|S|*|U|*|U| + 3*|S|*|U| + |U|*|U| + |S| + 4*|U| + 4;
   }
-  */
-  4*|I|*|I|*|U| + |I|*|S|*|U| + 4*|I|*|U| + |U|*|U| + |I| + 4*|U| + 4
+}
+
+lemma counter_simplification_special_case(U: set<int>, S: set<set<int>>, k: nat, I: set<set<int>>)
+  requires |I| <= |S|
+  ensures |U| + 1 + poly_isSubset(U, I, S) <= poly(U, S, k)
+{
+  calc <= {
+    |U| + 1 + poly_isSubset(U, I, S);
+    |U| + 1 + |I|*|I|*|U| + |I|*|S|*|U| + 2*|I|*|U| + |I| + 2;
+    |I|*|I|*|U| + |I|*|S|*|U| + 2*|I|*|U| + |U| + |I| + 3;
+    assert |I|*|S|*|U| <= |S|*|S|*|U| by {
+      mult_preserves_order(|I|, |U|*|S|, |S|, |U|*|S|);
+    }
+    |I|*|I|*|U| + |S|*|S|*|U| + 2*|S|*|U| + |U| + |S| + 3;
+    assert |I|*|I|*|U| <= |I|*|S|*|U| by {
+      mult_preserves_order(|I|, |I|*|U|, |S|, |I|*|U|);
+    }
+    |I|*|S|*|U| + |S|*|S|*|U| + 2*|S|*|U| + |U| + |S| + 3;
+    assert |I|*|S|*|U| <= |S|*|S|*|U| by {
+      mult_preserves_order(|I|, |S|*|U|, |S|, |S|*|U|);
+    }
+    |S|*|S|*|U| + |S|*|S|*|U| + 2*|S|*|U| + |U| + |S| + 3;
+    2*|S|*|S|*|U| + 2*|S|*|U| + |U| + |S| + 3;
+    |S|*|S|*|U|*|U| + 2*|S|*|S|*|U| + 3*|S|*|U|*|U| + 3*|S|*|U| + |U|*|U| + |S| + 4*|U| + 4;
+    poly(U, S, k);
+  }
 }
